Loogle/TrieProofs.lean
@@ -1,0 +1,186 @@
+import Loogle.Trie
+import Std.Data.ByteArray
+
+set_option autoImplicit false
+
+@[simp]
+axiom String.utf8ByteSize_eq_toUTF8_size (s : String) : s.utf8ByteSize = s.toUTF8.size
+
+axiom String.getUtf8Byte_eq_toUTF8_get (s : String) (i : Nat) (h : i < s.utf8ByteSize) :
+  s.getUtf8Byte i h = s.toUTF8.get ⟨i, s.utf8ByteSize_eq_toUTF8_size ▸ h⟩
+
+@[simp]
+theorem ByteArray.toList_mk (bs : Array UInt8) : (ByteArray.mk bs).toList = bs.toList := sorry
+
+@[simp]
+theorem ByteArray.toList_push (bs : ByteArray) (c : UInt8) :
+  (bs.push c).toList = bs.toList ++ [c] := sorry
+
+theorem ByteArray.size_list (bs : ByteArray) :
+  bs.size = bs.toList.length := sorry
+
+theorem ByteArray.findIdx_list (bs : ByteArray) (p : UInt8 → Bool) :
+  bs.findIdx? p = bs.toList.findIdx? p := sorry
+
+theorem ByteArray.get_list (bs : ByteArray) (i : Fin bs.size) :
+  bs.get i = bs.toList.get (i.cast (bs.size_list)) := sorry
+
+theorem List.nodup_snoc :
+  ∀ {α : Type _} {a : α} {l : List α}, List.Nodup (l ++ [a]) ↔ a ∉ l ∧ List.Nodup l := sorry
+
+theorem Array.get?_modify {α : Type _} (ts : Array α) (i j : Nat) (f : α → α) :
+  (ts.modify i f).get? j = (if i = j then (ts.get? i).map f else ts.get? j) := sorry
+
+open Loogle
+
+theorem Trie.commonPrefix_differs
+  (s₁ : String) (s₂ : ByteArray) (offset1 : Nat)
+  (h1 : offset1 + Trie.commonPrefix s₁ s₂ offset1 < s₁.utf8ByteSize)
+  (h2 : Trie.commonPrefix s₁ s₂ offset1 < s₂.size) :
+  s₁.getUtf8Byte (offset1 + Trie.commonPrefix s₁ s₂ offset1) h1
+    ≠ ByteArray.get! s₂ (Trie.commonPrefix s₁ s₂ offset1) := sorry
+
+theorem Trie.commonPrefix_differs_head
+  (s₁ : String) (s₂ : ByteArray) (offset1 : Nat)
+  (heq0 : Trie.commonPrefix s₁ s₂ offset1 = 0)
+  (h1 : offset1 < s₁.utf8ByteSize)
+  (h2 : 0 < s₂.size) :
+  s₁.getUtf8Byte offset1 h1 ≠ ByteArray.get! s₂ 0 := by
+    have := Trie.commonPrefix_differs s₁ s₂ offset1
+    simp only [heq0, Nat.add_zero] at this
+    apply this <;> assumption
+
+
+inductive Trie.valid {α} : Trie α → Prop
+  | leaf (v : Option α) : valid (.leaf v)
+  | path (v : Option α)
+    (ps : ByteArray) (hps : 0 < ps.size)
+    (t : Trie α) (ht : Trie.valid t) : valid (.path v ps t)
+  | node (v : Option α)
+    (cs : ByteArray)
+    (ts : Array (Trie α))
+    (hsize : cs.size = ts.size)
+    (hdistinct : cs.toList.Nodup)
+    (hts : ∀ t, t ∈ ts → Trie.valid t) : Trie.valid (Trie.node v cs ts)
+
+theorem valid_loop_insertEmpty {α} (i : Nat) (k : String) (f : Option α → α) :
+    Trie.valid (Trie.upsert.insertEmpty k f i) := by
+  unfold Trie.upsert.insertEmpty
+  split
+  case inl h =>
+    apply Trie.valid.path
+    · simp at *; omega
+    · apply Trie.valid.leaf
+  case inr h =>
+  · apply Trie.valid.leaf
+
+theorem valid_loop_upsert {α} (t : Trie α) (i : Nat) (k : String) (f : Option α → α) (h : Trie.valid t):
+    Trie.valid (Trie.upsert.loop k f i t) := by
+  cases h with
+  | leaf v =>
+    simp only [Trie.upsert.loop]
+    split
+    case inr hi => apply Trie.valid.leaf
+    case inl hi =>
+      constructor
+      · simp only [ByteArray.size_extract, String.utf8ByteSize_eq_toUTF8_size, Nat.min_self] at *
+        omega
+      · apply Trie.valid.leaf
+  | path v ps hps t ht =>
+    simp only [Trie.upsert.loop]
+    split
+    case inr hi => apply Trie.valid.path <;> assumption
+    case inl hi =>
+      split
+      case inl hp =>
+        apply Trie.valid.path
+        · simp only [ByteArray.size_extract, Nat.sub_zero, Nat.lt_min]
+          omega
+        · apply valid_loop_upsert -- induction happens here
+          split
+          case inl hp2 =>
+            apply Trie.valid.path
+            · simp only [ByteArray.size_extract, Nat.sub_pos_iff_lt, Nat.lt_min]
+              omega
+            · exact ht
+          case inr hp => exact ht
+      case inr hp =>
+        apply Trie.valid.node
+        · simp [ByteArray.size]
+        · have heq0 : Trie.commonPrefix k ps i = 0 := by omega
+          have := Trie.commonPrefix_differs_head k ps i heq0 hi hps
+          simpa [List.Nodup]
+        · simp only [List.mem_toArray, List.mem_cons, List.mem_singleton, forall_eq_or_imp, forall_eq]
+          constructor
+          case left =>
+            apply valid_loop_insertEmpty
+          case right =>
+            simp only [List.not_mem_nil, false_implies, forall_const, and_true]
+            split
+            case inl _ => exact ht
+            case inr hps1 =>
+              apply Trie.valid.path
+              · simp;omega
+              · exact ht
+  | node v cs ts hsize hdisitnct hts =>
+    simp only [Trie.upsert.loop]
+    split
+    case inr hi => apply Trie.valid.node <;> assumption
+    case inl hi =>
+      rw [ByteArray.findIdx_list]
+      split
+      case h_1 _ hfindnone =>
+        apply Trie.valid.node
+        · simpa
+        · simp only [ByteArray.toList_push, List.nodup_snoc, hdisitnct, and_true]
+          simp only [List.mem_iff_get?, not_exists]
+          intro j hj
+          have := List.findIdx?_of_eq_none hfindnone j
+          rw [hj] at this
+          simp at this
+          done
+        · simp only [← Array.mem_data, Array.push_data, List.mem_append, List.mem_singleton]
+          simp only [Array.mem_data]
+          intro t ht
+          cases ht with
+          | inl ht => exact hts t ht
+          | inr ht => cases ht; apply valid_loop_insertEmpty
+      case h_2 _ idx _hfindsome =>
+        apply Trie.valid.node
+        · simpa
+        · assumption
+        · simp only [← Array.mem_data, List.mem_iff_get?, forall_exists_index]
+          simp only [← Array.get?_eq_data_get?]
+          simp only [Array.get?_modify]
+          intro t' j
+          split
+          case inl hj =>
+            cases hj
+            simp only [Option.map_eq_some', forall_exists_index, and_imp]
+            intro t'' ht'' ht''
+            cases ht''
+            apply valid_loop_upsert -- induction happens here
+            apply hts
+            simp only [← Array.mem_data, List.mem_iff_get?]
+            simp only [← Array.get?_eq_data_get?]
+            exact ⟨_, ht''⟩
+          case inr hj =>
+            intro ht''
+            apply hts
+            simp only [← Array.mem_data, List.mem_iff_get?]
+            simp only [← Array.get?_eq_data_get?]
+            exact ⟨_, ht''⟩
+            done
+termination_by _ => k.utf8ByteSize - i
+decreasing_by
+  simp_wf
+  simp only [← String.utf8ByteSize_eq_toUTF8_size] at *
+  omega
+
+
+theorem valid_upsert {α} (t : Trie α) (k : String) (f : Option α → α) (h : Trie.valid t):
+  Trie.valid (t.upsert k f) := valid_loop_upsert _ _ _ _ h
+
+theorem find_upsert {α} (t : Trie α) (k₁ k₂ : String) (f : Option α → α) :
+    (t.upsert k₁ f).find? k₂ = (if k₂ = k₁ then some (f (t.find? k₂)) else t.find? k₂) := by
+  sorry
